lush/Crypto/BitOperations.lean
@@ -20,4 +20,55 @@ def toArrayBE (n : UInt32) : Array UInt8 :=
   ]
 
 theorem size_toArrayBE (n : UInt32) : n.toArrayBE.size = 4 := by simp [toArrayBE]
+
+def ofArrayBE (b : ByteArray) (h : b.size = 4) : UInt32 :=
+  (b[0].toUInt32 <<< 24)
+  ||| (b[1].toUInt32 <<< 16)
+  ||| (b[2].toUInt32 <<< 8)
+  ||| b[3].toUInt32
+
 end UInt32
+
+namespace Nat
+
+def toByteArray (n : Nat) : ByteArray :=
+  Id.run do
+    let mut b := ByteArray.empty
+    let mut n := n
+    while n > 0 do
+      let byte := (n &&& 0xFF).toUInt8
+      b := b.push byte
+      n := n >>> 8
+    return (b.data.reverse |> ByteArray.mk)
+
+def toHexDigit (n : Nat) : String :=
+  if n < 10 then toString n
+  else if n = 10 then "a"
+  else if n = 11 then "b"
+  else if n = 12 then "c"
+  else if n = 13 then "d"
+  else if n = 14 then "e"
+  else if n = 15 then "f"
+  else "-"
+
+def toHex (n : Nat) : String :=
+  Id.run do
+    let mut n := n
+    let mut s := []
+    while n > 0 do
+      s := (n % 16).toHexDigit :: s
+      n := n / 16
+    return String.join s
+
+end Nat
+
+namespace ByteArray
+
+def toNat (b : ByteArray) : Nat :=
+  Id.run do
+    let mut n := 0
+    for i in List.finRange b.size do
+      n := (n <<< 8) ||| b[i].toNat
+    n
+
+end ByteArray
