lush/Crypto/HMAC.lean
@@ -34,13 +34,13 @@ def sha256hmac (message : ByteArray) (key : ByteArray) : ByteArray :=
 -- Test vector 1:
 example :
     sha256hmac ("Hi There").toUTF8 (ByteArray.mk (Array.replicate 20 0x0b))
-    = natToByteArray 0xb0344c61d8db38535ca8afceaf0bf12b881dc200c9833da726e9376c2e32cff7 := by
+    = 0xb0344c61d8db38535ca8afceaf0bf12b881dc200c9833da726e9376c2e32cff7.toByteArray := by
   native_decide
 
 -- Test vector 2:
 example :
     sha256hmac "what do ya want for nothing?".toUTF8 "Jefe".toUTF8
-    = natToByteArray 0x5bdcc146bf60754e6a042426089575c75a003f089d2739839dec58b964ec3843 := by
+    = 0x5bdcc146bf60754e6a042426089575c75a003f089d2739839dec58b964ec3843.toByteArray := by
   native_decide
 
 -- Test vector 3:
@@ -50,7 +50,7 @@ example :
     sha256hmac
       (ByteArray.mk (Array.replicate 50 0xdd))
       (ByteArray.mk (Array.replicate 20 0xaa))
-    = natToByteArray 0x773ea91e36800e46854db8ebd09181a72959098b3ef8c122d9635514ced565fe := by
+    = 0x773ea91e36800e46854db8ebd09181a72959098b3ef8c122d9635514ced565fe.toByteArray := by
   native_decide
 
 -- Test vector 4:
@@ -64,7 +64,7 @@ example :
         0x0a, 0x0b, 0x0c, 0x0d, 0x0e, 0x0f, 0x10, 0x11, 0x12,
         0x13, 0x14, 0x15, 0x16, 0x17, 0x18, 0x19
       ])
-    = natToByteArray 0x82558a389a443c0ea4cc819899f2083a85f0faa3e578f8077a2e3ff46729665b := by
+    = 0x82558a389a443c0ea4cc819899f2083a85f0faa3e578f8077a2e3ff46729665b.toByteArray := by
   native_decide
 
 -- Test vector 5 (truncated output to 128 bits = first 16 bytes):
@@ -75,7 +75,7 @@ example :
       "Test With Truncation".toUTF8
       (ByteArray.mk (Array.replicate 20 0x0c))
     ).extract 0 16
-    = natToByteArray 0xa3b6167473100ee06e0c796c2955552b := by
+    = 0xa3b6167473100ee06e0c796c2955552b.toByteArray := by
   native_decide
 
 -- Test vector 6:
@@ -85,7 +85,7 @@ example :
     sha256hmac
       "Test Using Larger Than Block-Size Key - Hash Key First".toUTF8
       (ByteArray.mk (Array.replicate 131 0xaa))
-    = natToByteArray 0x60e431591ee0b67f0d8a26aacbf5b77f8e0bc6213728c5140546040f0ee37f54 := by
+    = 0x60e431591ee0b67f0d8a26aacbf5b77f8e0bc6213728c5140546040f0ee37f54.toByteArray := by
   native_decide
 
 -- Test vector 7:
@@ -95,7 +95,7 @@ example :
     sha256hmac
       "This is a test using a larger than block-size key and a larger than block-size data. The key needs to be hashed before being used by the HMAC algorithm.".toUTF8
       (ByteArray.mk (Array.replicate 131 0xaa))
-    = natToByteArray 0x9b09ffa71b942fcb27635fbcd5b0e944bfdc63644f0713938a7f51535c3a35e2 := by
+    = 0x9b09ffa71b942fcb27635fbcd5b0e944bfdc63644f0713938a7f51535c3a35e2.toByteArray := by
   native_decide
 
 end Lush.Crypto.HMAC
